finish (understanding, as there's no exercise) chapter 13, impparser.

vol1/impparser/defns.v
@@ -1,3 +1,11 @@
+(* This chapter has no exercises.
+I give myself my own exercises:
+	 1. understand what's going on inside the non-trivial constructs and comment
+	 them out.
+	 2. Figure out each type that is not explicitly given, and add them myself as
+	 type hints.
+ *)
+
 Set Warnings "-notation-overridden,-parsing,-deprecated-hint-without-locality".
 From Coq Require Import Strings.String.
 From Coq Require Import Strings.Ascii.
@@ -6,6 +14,7 @@ From Coq Require Import Init.Nat.
 From Coq Require Import EqNat.
 From Coq Require Import List. Import ListNotations.
 
+(* These are trivial, just comparing ascii values *)
 Definition isWhite (c : ascii) : bool :=
   let n := nat_of_ascii c in
   orb (orb (n =? 32) (* space *)
@@ -46,6 +55,17 @@ Definition token := string.
 
 From LF.maps Require Import maps.
 
+(*
+  A token is a consecutive subsequence of a string that has the
+  same chartype (excluding whitespace and '(' ')' ).
+  whitespaces are ignored while each of '(' and ')' is a token on its own.
+  cls is the type of the current token, initially set to whitespace.
+  acc is the accumulator building the current token, cleared and attached 
+  to the result as tk whenever cls changes or whenever '(' or ')' is 
+  encountered.
+
+	@returns a list of tokens.
+*)
 Fixpoint tokenize_helper (cls : chartype) (acc xs : list ascii)
                        : list (list ascii) :=
   let tk := match acc with [] => [] | _::_ => [rev acc] end in
@@ -77,3 +97,366 @@ Example tokenize_ex1 :
        "*"; "("; "3"; "+"; "(";
        "a"; "+"; "c"; ")"; ")"]%string.
 Proof. reflexivity. Qed.
+
+Inductive optionE (X:Type) : Type :=
+  | SomeE (x : X)
+  | NoneE (s : string).
+Arguments SomeE {X}.
+Arguments NoneE {X}.
+
+
+(* 
+	This is confusing at first glance. What does it do?
+	Turns out that it is used to treat optionE as much as we can like a normal
+	 variable. p is the variable inside e1, and will be used as is in e2.
+	For example,
+	' y <-
+		' x <- e1 ;; optionE (x+1)
+	;; optionE (y+1)
+	is to have e1's variable +1 +1.
+*)
+Notation "' p <- e1 ;; e2"
+   := (match e1 with
+       | SomeE p => e2
+       | NoneE err => NoneE err
+       end)
+   (right associativity, p pattern, at level 60, e1 at next level).
+
+Notation "'TRY' e1 'OR' e2"
+   := (
+    let result := e1 in
+    match result with
+       | SomeE _ => result
+       | NoneE _ => e2
+       end)
+   (right associativity,
+    at level 60, e1 at next level, e2 at next level).
+
+Open Scope string_scope.
+
+(* A parse seems to me is a function that parses the head token in a list
+	 into type T.
+ *)
+Definition parser (T : Type) :=
+  list token -> optionE (T * list token).
+
+(* Seems to me to be a parsing helper that requires the parsing to be done
+ * within steps and repeatedly invokes parser until
+	 1. parsing terminates with NoneE, either because of a parsing error or
+	 because xs becomes empty.
+	 2. steps have been exhausted.
+
+	 Its return type is unspecified, and it should be
+	 optionE ( (list T) * (list token) ), where
+	 list T is the parsed types and list token is the remaining ones.
+
+	There are a few issues here:
+	1. when steps is reached, all progress is lost as NoneE is returned.
+	I would have to return the current progress so far.
+	2. the second match clause _, NoneE _ seems to intend to capture parsing end:
+	when xs = [], a parser should return NoneE. However, if the parsing fails on
+	a xs != [], then the parser might return NoneE as well, and there's no way to
+	tell.
+ *)
+Fixpoint many_helper {T} 
+	(p : parser T) 
+	(acc : list T)
+	(steps : nat)
+	(xs : list token) 
+	: optionE ( (list T) * (list token) )
+	:=
+  match steps, p xs with
+  | 0, _ =>
+      NoneE "Too many recursive calls"
+  | _, NoneE _ =>
+      SomeE ((rev acc), xs)
+  | S steps', SomeE (t, xs') =>
+      many_helper p (t :: acc) steps' xs'
+  end.
+
+(* 
+	This thus defines a parser that, instead of 
+	parsing only the head of a list, parses ... at most steps-1 elements.	
+	This is because at step NoneE is returned, as mentioned earlier.
+
+	This makes the procedure either
+	1. parses the input entirely, where len(input) < steps
+	2. or fail entirely with NoneE "Too many recursive calls"
+	3. or on rare cases, abort because a parsing error has occurred, which we
+	 don't know about unless we check the len(output) < len(input).
+
+	contrary to the natural idea that many parses the first steps of the tokens.
+	That is not true.
+*)
+Definition many {T} (p : parser T) (steps : nat) : parser (list T) :=
+  many_helper p [] steps.
+
+(* First expects the first token is t.
+If so, then apply p to the rest.
+	 Otherwise, return NoneE *)
+Definition firstExpect {T} (t : token) (p : parser T)
+                     : parser T :=
+  fun xs => match xs with
+            | x::xs' =>
+              if string_dec x t
+              then p xs'
+              else NoneE ("expected '" ++ t ++ "'.")
+            | [] =>
+              NoneE ("expected '" ++ t ++ "'.")
+            end.
+
+Definition expect (t : token) : parser unit :=
+  firstExpect t (fun xs => SomeE (tt, xs)).
+
+
+(* An identifier can only be lower alpha *)
+Definition parseIdentifier (xs : list token)
+                         : optionE (string * list token) :=
+match xs with
+| [] => NoneE "Expected identifier"
+| x::xs' =>
+    if forallb isLowerAlpha (list_of_string x) then
+      SomeE (x, xs')
+    else
+      NoneE ("Illegal identifier:'" ++ x ++ "'")
+end.
+
+(* the digit parsing function is a common way to parse an integer *)
+Definition parseNumber (xs : list token)
+                     : optionE (nat * list token) :=
+match xs with
+| [] => NoneE "Expected number"
+| x::xs' =>
+    if forallb isDigit (list_of_string x) then
+      SomeE (fold_left
+               (fun n d =>
+                  10 * n + (nat_of_ascii d -
+                            nat_of_ascii "0"%char))
+               (list_of_string x)
+               0,
+             xs')
+    else
+      NoneE "Expected number"
+end.
+
+From LF.imp Require Import defns.
+
+(* either an identifier, a canonical number,
+	 or a non-carnonical expression enclosed in ( ),
+	 in which case that expression will be evaluated and its value will act as
+	 the parsed result *)
+Fixpoint parsePrimaryExp (steps:nat)
+                         (xs : list token)
+                       : optionE (aexp * list token) :=
+  match steps with
+  | 0 => NoneE "Too many recursive calls"
+  | S steps' =>
+      TRY ' (i, rest) <- parseIdentifier xs ;;
+          SomeE (AId i, rest)
+      OR
+      TRY ' (n, rest) <- parseNumber xs ;;
+          SomeE (ANum n, rest)
+      OR
+      ' (e, rest) <- firstExpect "(" (parseSumExp steps') xs ;;
+      ' (u, rest') <- expect ")" rest ;;
+      SomeE (e,rest')
+  end
+
+(* First checks if the first few tokens form a primary exp.
+	If so, then parse its value as e.
+	2. Then, see if the next token is '*'. If not, fail.
+	3. If so, then parse the rest as primary exp, stored in es. 
+	2 and 3 are repeated for many times until the expression is exhausted.
+	All the result primary exps are stored in list es, and fold_left is done on
+	 AMult es e. The order is correct, e.g., fold_left AMult [b, c] a = 
+	 AMult (AMult a b) c, which is the result of parsing a*b*c
+	 (left-associativity).
+*)
+with parseProductExp (steps:nat)
+                     (xs : list token) :=
+  match steps with
+  | 0 => NoneE "Too many recursive calls"
+  | S steps' =>
+    ' (e, rest) <- parsePrimaryExp steps' xs ;;
+    ' (es, rest') <- many (firstExpect "*" (parsePrimaryExp steps'))
+                          steps' rest ;;
+    SomeE (fold_left AMult es e, rest')
+  end
+(* This has the same idea of parseProductExp, but 
+	 has to handle both + and - and thus has to also include a boolean to
+	 indicate that. *)
+with parseSumExp (steps:nat) (xs : list token) :=
+  match steps with
+  | 0 => NoneE "Too many recursive calls"
+  | S steps' =>
+    ' (e, rest) <- parseProductExp steps' xs ;;
+    ' (es, rest') <-
+        many (fun xs =>
+                TRY ' (e,rest') <-
+                    firstExpect "+"
+                                (parseProductExp steps') xs ;;
+                    SomeE ( (true, e), rest')
+                OR
+                ' (e, rest') <-
+                    firstExpect "-"
+                                (parseProductExp steps') xs ;;
+                SomeE ( (false, e), rest'))
+        steps' rest ;;
+      SomeE (fold_left (fun e0 term =>
+                          match term with
+                          | (true, e) => APlus e0 e
+                          | (false, e) => AMinus e0 e
+                          end)
+                       es e,
+             rest')
+  end.
+Definition parseAExp := parseSumExp.
+(* we just need to handle a lot of cases here.
+The basic idea is still the same as in primary exp:
+if in ( ), then parse the expr inside as the most general form.
+Otherwise, proceed normally.
+ *)
+Fixpoint parseAtomicExp (steps:nat)
+                        (xs : list token) :=
+match steps with
+  | 0 => NoneE "Too many recursive calls"
+  | S steps' =>
+     TRY ' (u,rest) <- expect "true" xs ;;
+         SomeE (BTrue,rest)
+     OR
+     TRY ' (u,rest) <- expect "false" xs ;;
+         SomeE (BFalse,rest)
+     OR
+     TRY ' (e,rest) <- firstExpect "~"
+                                   (parseAtomicExp steps')
+                                   xs ;;
+         SomeE (BNot e, rest)
+     OR
+     TRY ' (e,rest) <- firstExpect "("
+                                   (parseConjunctionExp steps')
+                                   xs ;;
+         ' (u,rest') <- expect ")" rest ;;
+         SomeE (e, rest')
+     OR
+     ' (e, rest) <- parseProductExp steps' xs ;;
+     TRY ' (e', rest') <- firstExpect "="
+                                  (parseAExp steps') rest ;;
+         SomeE (BEq e e', rest')
+     OR
+     TRY ' (e', rest') <- firstExpect "<="
+                                      (parseAExp steps') rest ;;
+         SomeE (BLe e e', rest')
+     OR
+     NoneE "Expected '=' or '<=' after arithmetic expression"
+end
+
+(* Similar to parseProductExp *)
+with parseConjunctionExp (steps:nat)
+                         (xs : list token) :=
+  match steps with
+  | 0 => NoneE "Too many recursive calls"
+  | S steps' =>
+    ' (e, rest) <- parseAtomicExp steps' xs ;;
+    ' (es, rest') <- many (firstExpect "&&"
+               (parseAtomicExp steps'))
+            steps' rest ;;
+    SomeE (fold_left BAnd es e, rest')
+  end.
+Definition parseBExp := parseConjunctionExp.
+Check parseConjunctionExp.
+Definition testParsing {X : Type}
+           (p : nat ->
+                list token ->
+                optionE (X * list token))
+           (s : string) :=
+  let t := tokenize s in
+  p 100 t.
+(* Based on the syntax, we will be able to expect which type of expr
+	 (boolean, primary, etc.) will the next be.
+	 Then, proceed accordingly *)
+Fixpoint parseSimpleCommand (steps:nat)
+                            (xs : list token) :=
+  match steps with
+  | 0 => NoneE "Too many recursive calls"
+  | S steps' =>
+    TRY ' (u, rest) <- expect "skip" xs ;;
+        SomeE (<{skip}>, rest)
+    OR
+    TRY ' (e,rest) <-
+            firstExpect "if"
+                        (parseBExp steps') xs ;;
+        ' (c,rest') <-
+            firstExpect "then"
+                        (parseSequencedCommand steps') rest ;;
+        ' (c',rest'') <-
+            firstExpect "else"
+                        (parseSequencedCommand steps') rest' ;;
+        ' (tt,rest''') <-
+            expect "end" rest'' ;;
+       SomeE(<{if e then c else c' end}>, rest''')
+    OR
+    TRY ' (e,rest) <-
+            firstExpect "while"
+                        (parseBExp steps') xs ;;
+        ' (c,rest') <-
+            firstExpect "do"
+                        (parseSequencedCommand steps') rest ;;
+        ' (u,rest'') <-
+            expect "end" rest' ;;
+        SomeE(<{while e do c end}>, rest'')
+    OR
+    TRY ' (i, rest) <- parseIdentifier xs ;;
+        ' (e, rest') <- firstExpect ":=" (parseAExp steps') rest ;;
+        SomeE (<{i := e}>, rest')
+    OR
+        NoneE "Expecting a command"
+end
+
+with parseSequencedCommand (steps:nat)
+                           (xs : list token) :=
+  match steps with
+  | 0 => NoneE "Too many recursive calls"
+  | S steps' =>
+    ' (c, rest) <- parseSimpleCommand steps' xs ;;
+    TRY ' (c', rest') <-
+            firstExpect ";"
+                        (parseSequencedCommand steps') rest ;;
+        SomeE (<{c ; c'}>, rest')
+    OR
+    SomeE (c, rest)
+  end.
+Definition bignumber := 1000.
+Definition parse (str : string) : optionE com :=
+  let tokens := tokenize str in
+  match parseSequencedCommand bignumber tokens with
+  | SomeE (c, []) => SomeE c
+  | SomeE (_, t::_) => NoneE ("Trailing tokens remaining: " ++ t)
+  | NoneE err => NoneE err
+  end.
+
+Example eg1 : parse " if x = y + 1 + 2 - y * 6 + 3 then x := x * 1; y := 0 else skip end "
+=
+  SomeE <{
+      if ("x" = ("y" + 1 + 2 - "y" * 6 + 3)) then
+        "x" := "x" * 1;
+        "y" := 0
+      else
+        skip
+      end }>.
+Proof. cbv. reflexivity. Qed.
+Example eg2 : parse " skip; z:=x*y*(x*x); while x=x do if (z <= z*z) && ~(x = 2) then x := z; y := z else skip end; skip end; x:=z "
+=
+  SomeE <{
+      skip;
+      "z" := "x" * "y" * ("x" * "x");
+      while ("x" = "x") do
+        if ("z" <= "z" * "z") && ~("x" = 2) then
+          "x" := "z";
+          "y" := "z"
+        else
+          skip
+        end;
+        skip
+      end;
+      "x" := "z" }>.
+Proof. cbv. reflexivity. Qed.
